aneris/examples/reliable_communication/lib/repdb/proof/follower/proof_of_sync_loop.v
@@ -1,0 +1,157 @@
+From iris.algebra.lib Require Import mono_list.
+From iris.base_logic Require Import invariants.
+From iris.bi.lib Require Import fractional.
+From iris.proofmode Require Import tactics coq_tactics reduction spec_patterns.
+From aneris.lib Require Import gen_heap_light.
+From aneris.aneris_lang Require Import lang resources inject tactics proofmode.
+From aneris.aneris_lang.lib Require Import
+     list_proof monitor_proof lock_proof map_proof assert_proof.
+From aneris.aneris_lang.lib.serialization Require Import serialization_proof.
+From aneris.aneris_lang.program_logic Require Import aneris_lifting.
+From aneris.aneris_lang.program_logic Require Import aneris_weakestpre.
+From aneris.examples.reliable_communication.prelude
+     Require Import ser_inj.
+From aneris.examples.reliable_communication.lib.mt_server
+     Require Import user_params mt_server_code.
+From aneris.examples.reliable_communication.lib.mt_server.spec
+     Require Import api_spec.
+From aneris.examples.reliable_communication.lib.repdb
+     Require Import repdb_code model.
+From aneris.examples.reliable_communication.lib.repdb.spec
+     Require Import db_params time events resources.
+From aneris.examples.reliable_communication.lib.repdb.resources
+     Require Import
+     ras log_resources resources_def
+     resources_global_inv resources_local_inv.
+From aneris.examples.reliable_communication.lib.repdb.proof
+     Require Import
+     repdb_serialization log_proof.
+From aneris.examples.reliable_communication.lib.repdb.proof.leader
+     Require Import
+     followers_mt_user_params.
+
+Import log_proof.
+
+Section SyncLogCopy_Proof.
+  Context `{!anerisG Mdl Σ, dbparams : !DB_params, !IDBG Σ}.
+  Context (γL γM γF : gname) ( sa : socket_address) (kvsL logL : loc).
+
+  Global Instance MTU : MTS_user_params.
+  Proof. apply (follower_handler_user_params γL γM). Defined.
+
+ Definition own_replog_loop l : iProp Σ :=
+    known_replog_token sa γF ∗ own_replog_obs γL DB_addrF l ∗
+    own_log_auth γF (1/4) l.
+
+  Lemma sync_loop_spec
+        (mγ : gname) (mv : val) (reqh : val) (logM : wrlog) (n : nat) :
+    n = length logM →
+    {{{ Global_Inv γL γM ∗
+        follower_local_inv γL kvsL logL sa γF mγ mv ∗
+        make_request_spec reqh sa ∗
+        own_replog_loop logM
+    }}}
+      sync_loop #kvsL #logL mv reqh #n @[ip_of_address sa]
+    {{{ RET #(); True }}}.
+  Proof.
+    iIntros (Hn Φ) "(#HGinv & #HinvL & #Hreqh & HlogM) HΦ".
+    rewrite /sync_loop. do 12 wp_pure _.
+    iLöb as "IH" forall (n logM Hn).
+    iDestruct "HlogM" as "(#Hknw & #HobsL & HlogM)".
+    iDestruct (get_obs with "[$HlogM]") as "#HobsF".
+    wp_pures. rewrite /make_request_spec. wp_apply ("Hreqh" $! _ logM).
+    { iSplit; first by iPureIntro; apply _. iFrame "#"; naive_solver. }
+    iIntros (logM' repv) "Hpost".
+    iDestruct "Hpost" as (we) "(-> & %Hlen & -> & #HobsLF')".
+    do 13 wp_pure _.
+    rewrite Hlen Hn.
+    wp_apply wp_assert.
+    wp_pures. iSplit.
+    { iPureIntro. by case_bool_decide. }
+    iNext. wp_pures.
+    wp_apply (monitor_acquire_spec with "[HinvL]"); first by iFrame "#".
+    iIntros (v) "( -> & Hlocked & Hres)".
+    wp_pures.
+   (*iDestruct "Hres" as (logV logM) "(%Hlog & Hpl & HmainLog & HmainRes)".
+    iAssert (⌜lF `prefix_of` logM⌝)%I as "%Hprefix".
+    { iDestruct "Hloop" as "(_ & Hobs & _)".
+      iApply (own_obs_prefix with "[$HmainLog][$Hobs]"). }
+    assert (length lF ≤ length logM) as Hlen2.
+    { by apply prefix_length. }
+    wp_apply (wp_log_wait_until
+               with "[$HinvL $Hlocked $Hpl $HmainLog $HmainRes][Hloop HΦ]").
+    { naive_solver. }
+    iNext.
+    iIntros (logV' logM').
+    iIntros "(%Hlen' & %Hlog' & Hlocked & HmainRes & Hpl & HmainLog)".
+    wp_pures.
+    wp_load.
+    wp_pures.
+    iAssert (⌜lF `prefix_of` logM'⌝)%I as "%Hprefix2".
+    {  iDestruct "Hloop" as "(_ & Hobs & _)".
+       by iDestruct (own_obs_prefix with "[$HmainLog][$Hobs]") as "%Hprefix2". }
+    iDestruct (get_obs with "[$HmainLog]") as "#HobsM'".
+    wp_apply (monitor_release_spec
+               with "[$HinvL $Hlocked Hpl HmainLog HmainRes]").
+    iExists _, _. eauto with iFrame.
+    iIntros (v ->).
+    wp_pures.
+    rewrite HipEq.
+    wp_apply (monitor_acquire_spec with "[$HinvF]").
+    iIntros (v) "( -> & Hlocked & Hres)".
+    wp_pures.
+    iDestruct "Hres" as (logVF logMF) "(%HlogF & HplF & HLogOwnF & HResF)".
+    wp_store.
+    iDestruct "Hloop" as "(#HknownTkn & #Hobs & HownLoop)".
+    iDestruct (own_log_auth_combine
+                with "[$HLogOwnF][$HownLoop]") as "(HownFHalf1 & ->)".
+    assert (length lF < length logM') by lia.
+    clear logM Hlog Hprefix logV n Hlen Hlen' Hlen2.
+    rewrite /Global_Inv /global_inv_def.
+    iApply fupd_aneris_wp.
+    iInv DB_InvName as ">HGinvRes" "Hcl".
+    iDestruct "HGinvRes" as (L M N Hkes) "HGinvRes".
+    iDestruct "HGinvRes" as "(HownS & HownL & HknownN & HmapN & %HvSt)".
+    iAssert (⌜N !! DB_addrF = Some γF⌝)%I as "%HinF".
+    by iDestruct (known_replog_in_N with "[$HknownN $HknownTkn]") as "%HinN".
+    iDestruct (big_sepM_lookup_acc _ N DB_addrF γF with "[$HmapN]")
+      as "(Hres & HmapN)"; [done|].
+    iDestruct "Hres" as (l) "(#HknownTkn' & #Hobs' & HownFHalf2)".
+    iDestruct (own_log_auth_combine
+                with "[$HownFHalf1][$HownFHalf2]") as "(HownF & ->)".
+    rewrite Qp_quarter_quarter Qp_half_half.
+    iMod (own_log_auth_update _ l logM'
+           with "[$HownF]") as "HownF"; first done.
+    rewrite -Qp_half_half.
+    rewrite {1} Qp_half_half.
+    iDestruct (own_log_auth_split with "HownF") as "[HownF1 HownF2]".
+    rewrite -Qp_quarter_quarter.
+    rewrite {1} Qp_quarter_quarter.
+    iMod ("Hcl" with "[HownF1 HmapN HknownN HownS HownL]") as "_".
+    { iNext. iExists L, M, N. iFrame "#∗".
+      iSplit; first done.
+      iSplit; last done.
+      iApply "HmapN".
+      iExists logM'. iFrame "#∗". }
+    iModIntro.
+    iDestruct (own_log_auth_split with "HownF2") as "[HownF1 HownF2]".
+    wp_apply (monitor_broadcast_spec
+               with "[$HinvF $Hlocked HplF HResF HownF1]").
+    { iExists _, logM'.
+      rewrite /leader_local_secondary_res.
+      iFrame "#∗".
+      done. }
+    iIntros "(Hlocked & Hres)".
+    wp_pures.
+    wp_apply (monitor_release_spec with "[$HinvF $Hlocked $Hres]").
+    iIntros (v ->).
+    do 4 wp_pure _.
+    assert (∃ lV : val, logV' = (lV, #(length logM'))%V ∧ is_list logM' lV)
+           as (lV & -> & Hlst') by done.
+    do 1 wp_pure _.
+    iApply ("IH" $! logM' with "[//][$HΦ][$HownF2]").
+    iFrame "#∗".
+  Qed. *)
+  Admitted.
+
+End SyncLogCopy_Proof.
